# baseURI: http://loop3d.org/GSO/ontology/2020/1/quality/ontology
# imports: http://loop3d.org/GSO/ontology/2020/1/common/ontology

@prefix : <http://loop3d.org/GSO/ontology/2020/1/quality/> .
@prefix gsoc: <http://loop3d.org/GSO/ontology/2020/1/common/> .
@prefix gsoq: <http://loop3d.org/GSO/ontology/2020/1/quality/> .
@prefix owl: <http://www.w3.org/2002/07/owl#> .
@prefix rdf: <http://www.w3.org/1999/02/22-rdf-syntax-ns#> .
@prefix rdfs: <http://www.w3.org/2000/01/rdf-schema#> .
@prefix dct: <http://purl.org/dc/terms/> .
@prefix xsd: <http://www.w3.org/2001/XMLSchema#> .

gsoq:Colour
  rdf:type owl:Class ;
  rdfs:comment "upper level class that represents any conceptual space for quantifying colour, e.g. RGB, Munsell, CMYK, US NBS Color (NBS Special Pub 440)"@en ;
  rdfs:label "Colour"@en ;
  rdfs:subClassOf gsoc:Physical_Quality ;
  rdfs:subClassOf [
      rdf:type owl:Restriction ;
      owl:allValuesFrom gsoc:Material_Endurant ;
      owl:onProperty gsoc:isQualityOf ;
    ] ;
.
gsoq:Density
  rdf:type owl:Class ;
  rdfs:comment "The mass per unit volume of an Amount of Matter"@en ;
  rdfs:label "Density "@en ;
  rdfs:subClassOf gsoc:Physical_Quality ;
.
gsoq:Diameter
  rdf:type owl:Class ;
  rdfs:comment "The (approximate) average length of line segments that pass through the center of an object and whose endpoints lie on the outside boundary of the object. Use to characterize the size of a broadly spheroidal object like a pluton or a rock sample."@en ;
  rdfs:label "Diameter "@en ;
  rdfs:subClassOf gsoc:Physical_Quality ;
.
gsoq:Distance
  rdf:type owl:Class ;
  rdfs:comment "A measure of distance between locations"@en ;
  rdfs:label "Distance"@en ;
  rdfs:subClassOf gsoc:Physical_Quality ;
.
gsoq:Displacement
  rdf:type owl:Class ;
  rdfs:comment "A measure of change of location"@en ;
  rdfs:label "Displacement"@en ;
  rdfs:subClassOf gsoc:Physical_Quality ;
.
gsoq:Disseminated
  rdf:type owl:Class ;
  rdfs:comment "Quality is scattered relatively uniformly through the quality carrier."@en ;
  rdfs:label "Disseminated "@en ;
  rdfs:subClassOf gsoq:Distribution_Value ;
.
gsoq:Distribution
  rdf:type owl:Class ;
  rdfs:comment "spcification of how much of the quality carrier displays the quality. Use to indicate variability of development of the quality "@en ;
  rdfs:label "Quality distribution"@en ;
  rdfs:subClassOf gsoc:Nonphysical_Quality ;
  rdfs:subClassOf [
      rdf:type owl:Restriction ;
      owl:allValuesFrom gsoc:Quality ;
      owl:onProperty gsoc:isQualityOf ;
    ] ;
.
gsoq:Distribution_Value
  rdf:type owl:Class ;
  rdfs:comment "spcification of how much of the quality carrier displays the quality. Use to indicate variability of development of the quality "@en ;
  rdfs:label "Distribution Value"@en ;
  rdfs:subClassOf gsoc:Named_Value ;
  rdfs:subClassOf [
      rdf:type owl:Restriction ;
      owl:allValuesFrom gsoq:Distribution ;
      owl:onProperty gsoc:isValueOf ;
    ] ;
  rdfs:subClassOf [
      rdf:type owl:Restriction ;
      owl:onClass gsoq:Distribution ;
      owl:onProperty gsoc:isValueOf ;
      owl:qualifiedCardinality "1"^^xsd:nonNegativeInteger ;
    ] ;
.
gsoq:Intensity
  rdf:type owl:Class ;
  rdfs:comment "Intensity of quality "@en ;
  rdfs:label "Intensity Value"@en ;
  rdfs:subClassOf gsoc:Nonphysical_Quality ;
  rdfs:subClassOf [
      rdf:type owl:Restriction ;
      owl:allValuesFrom gsoc:Quality ;
      owl:onProperty gsoc:isQualityOf ;
    ] ;
.
gsoq:Intensity_Value
  rdf:type owl:Class ;
  rdfs:comment "Value of Intensity quality "@en ;
  rdfs:label "Value of Intensity quality "@en ;
  rdfs:subClassOf gsoc:Named_Value ;
  rdfs:subClassOf [
      rdf:type owl:Restriction ;
      owl:allValuesFrom gsoq:Intensity ;
      owl:onProperty gsoc:isValueOf ;
    ] ;
  rdfs:subClassOf [
      rdf:type owl:Restriction ;
      owl:onClass gsoq:Intensity ;
      owl:onProperty gsoc:isValueOf ;
      owl:qualifiedCardinality "1"^^xsd:nonNegativeInteger ;
    ] ;
.
gsoq:Layered_Distribution
  rdf:type owl:Class ;
  rdfs:comment "quality is exhibited in sheet like zones, e.g. along veins or fractures."@en ;
  rdfs:label "Layered distribution "@en ;
  rdfs:subClassOf gsoq:Distribution_Value ;
.

gsoq:Moderate_Intensity
  rdf:type owl:Class ;
  rdfs:comment "Quality is present and can be discerned by any observer"@en ;
  rdfs:label "moderate development" ;
  rdfs:subClassOf gsoq:Intensity_Value ;
.
gsoq:Orientation
  rdf:type owl:Class ;
  rdfs:comment "quality used to specify the disposition of a line or plane in space"@en ;
  rdfs:label "Orientation"@en ;
  rdfs:subClassOf gsoc:Physical_Quality ;
.
gsoq:Orientation_Value
  rdf:type owl:Class ;
  rdfs:subClassOf gsoc:Named_Value ;
  rdfs:subClassOf [
      rdf:type owl:Restriction ;
      owl:allValuesFrom gsoq:Orientation ;
      owl:onProperty gsoc:isValueOf ;
    ] ;
  rdfs:subClassOf [
      rdf:type owl:Restriction ;
      owl:onClass gsoq:Orientation ;
      owl:onProperty gsoc:isValueOf ;
      owl:qualifiedCardinality "1"^^xsd:nonNegativeInteger ;
    ] ;
.
gsoq:Patchy_Distribution
  rdf:type owl:Class ;
  rdfs:comment "Quality is exhibited in local concentrations separated by regions without the quality. Typically used to describe alteration distribution."@en ;
  rdfs:isDefinedBy "GeoSciML v4"@en ;
  rdfs:label "Patchy distribution"@en ;
  rdfs:subClassOf gsoq:Distribution_Value ;
.
gsoq:Pressure
  rdf:type owl:Class ;
  rdfs:comment "applies to Earth_Material or Geologic_Unit"@en ;
  rdfs:comment "peak metamorphic pressure"@en ;
  rdfs:isDefinedBy "GeoSciML v3"@en ;
  rdfs:label "Pressure"@en ;
  rdfs:subClassOf gsoc:Physical_Quality ;
.

gsoq:Sparse_Distribution
  rdf:type owl:Class ;
  rdfs:comment "Quality is occasionally present in instances of the host particular "@en ;
  rdfs:label "sparse distribution" ;
  rdfs:subClassOf gsoq:Distribution_Value ;
.
gsoq:Strong_Intensity
  rdf:type owl:Class ;
  rdfs:comment "Quality is present and is dominate feature of the quality host." ;
  rdfs:label "strong development" ;
  rdfs:subClassOf gsoq:Intensity_Value ;
.

gsoq:Temperature
  rdf:type owl:Class ;
  rdfs:comment "Temperature"@en ;
  rdfs:comment "applies to Earth_Material or Geologic_Unit"@en ;
  rdfs:isDefinedBy "GeoSciML v3"@en ;
  rdfs:label "Peak temperature"@en ;
  rdfs:subClassOf gsoc:Physical_Quality ;
.
gsoq:Thickness
  rdf:type owl:Class ;
  rdfs:comment "Quality of a tabular or sheet like body that is its linear dimension normal to its long dimensions. Could be quantified numerically or categorically (e.g. thin, thick, very thick)"@en ;
  rdfs:label "Thickness"@en ;
  rdfs:subClassOf gsoc:Physical_Quality ;
.
gsoq:Ubiquitous_Distribution
  rdf:type owl:Class ;
  rdfs:comment "Quality is everywhere present in the host."@en ;
  rdfs:label "ubiquitous distribution"@en ;
  rdfs:subClassOf gsoq:Distribution_Value ;
.
gsoq:Variable_Distribution
  rdf:type owl:Class ;
  rdfs:comment "Quality is not present to the same degree in all instances of the host particular"@en ;
  rdfs:label "variable distribution"@en ;
  rdfs:subClassOf gsoq:Distribution_Value ;
.
gsoq:Variable_Intensity
  rdf:type owl:Class ;
  rdfs:comment "Intensity varies spatially "@en ;
  rdfs:label "Variable intensity "@en ;
  rdfs:subClassOf gsoq:Intensity_Value ;
.
gsoq:Volume
  rdf:type owl:Class ;
  rdfs:comment "Volume of something occupying space"@en ;
  rdfs:label "Volume"@en ;
  rdfs:subClassOf gsoc:Physical_Quality ;
.
gsoq:Weak_Intensity
  rdf:type owl:Class ;
  rdfs:comment "Quality is present but difficult to discern "@en ;
  rdfs:label "weak development"@en ;
  rdfs:subClassOf gsoq:Intensity_Value ;
.
gsoq:ontology
  rdf:type owl:Ontology ;
  rdfs:comment "Vocabulary of physical qualities used in multiple GSO modules."@en ;
  rdfs:label "Physical qualities"@en ;
  owl:imports gsoc:ontology ;
.
