# baseURI: http://loop3d.org/GSO/ontology/2020/1/geologicfault/ontology
# imports: http://loop3d.org/GSO/ontology/2020/1/common/ontology
# imports: http://loop3d.org/GSO/ontology/2020/1/geology/ontology
# imports: http://loop3d.org/GSO/ontology/2020/1/quality/ontology
# imports: http://loop3d.org/GSO/ontology/2020/1/geologicquality/ontology
# imports: http://loop3d.org/GSO/ontology/2020/1/geologicprocess/ontology
# imports: http://loop3d.org/GSO/ontology/2020/1/geologicstructure/ontology

@prefix : <http://loop3d.org/GSO/ontology/2020/1/geologicfault/> .
@prefix gsfa: <http://loop3d.org/GSO/ontology/2020/1/geologicfault/> .
@prefix gsoc: <http://loop3d.org/GSO/ontology/2020/1/common/> .
@prefix gsog: <http://loop3d.org/GSO/ontology/2020/1/geology/> .
@prefix gsoq: <http://loop3d.org/GSO/ontology/2020/1/quality/> .
@prefix gsgq: <http://loop3d.org/GSO/ontology/2020/1/geologicquality/> .
@prefix gspr: <http://loop3d.org/GSO/ontology/2020/1/geologicprocess/> .
@prefix gsos: <http://loop3d.org/GSO/ontology/2020/1/geologicstructure/> .

@prefix owl: <http://www.w3.org/2002/07/owl#> .
@prefix rdf: <http://www.w3.org/1999/02/22-rdf-syntax-ns#> .
@prefix rdfs: <http://www.w3.org/2000/01/rdf-schema#> .
@prefix dct: <http://purl.org/dc/terms/> .
@prefix xsd: <http://www.w3.org/2001/XMLSchema#> .

gsfa:Detachment_Fault
  rdf:type owl:Class ;
  rdfs:comment "A regional-scale, large displacement, low-angle normal fault."@en ;
  dct:source  "CGI faulttype SKOS vocabulary 2016-10-19"@en ;
  rdfs:label "detachment fault"@en ;
  rdfs:subClassOf gsfa:Low_Angle_Normal_Fault ;
.
gsfa:Dextral_Strike_Slip_Fault
  rdf:type owl:Class ;
  rdfs:comment "Fault with right-lateral strike-parallel displacement component of slip vector more than 10 times the dip-parallel component of the slip vector at at least one location along the fault, and right-lateral displacement over more than half the mapped trace of the fault."@en ;
  dct:source  "CGI faulttype SKOS vocabulary 2016-10-19"@en ;
  rdfs:label "dextral strike slip fault"@en ;
  rdfs:subClassOf gsfa:Strike_Slip_Fault ;
.
gsfa:Dip_Separation
  rdf:type owl:Class ;
  rdfs:comment "A fault along which there is some separation parallel to the dip of the fault."@en ;
  dct:source  "GGIC vocabularies working group (Australia)"@en ;
  rdfs:label "dip separation sense"@en ;
  rdfs:subClassOf gsfa:Fault_Separation ;
.
gsfa:Dip_Slip
  rdf:type owl:Class ;
  rdfs:comment "The net slip of the fault lies in the dip direction of the fault."@en ;
  dct:source  "GGIC vocabularies working group (Australia)"@en ;
  rdfs:label "dip slip"@en ;
  rdfs:subClassOf gsfa:Fault_Slip ;
.
gsfa:Ductile_Shear_Zone
  rdf:type owl:Class ;
  rdfs:comment "a broadly planar zone of shear displacement within which deformation has occurred without loss of material continuity"@en ;
  rdfs:label "Ductile Shear Zone"@en ;
  rdfs:subClassOf gsfa:Fault_Zone ;
  rdfs:subClassOf [
      rdf:type owl:Restriction ;
      owl:onProperty gsoc:hasEssentialPart ;
      owl:someValuesFrom [
          rdf:type owl:Class ;
          owl:intersectionOf (
              gsog:Rock_Body
              [
                rdf:type owl:Restriction ;
                owl:onProperty gsoc:isOutputOf ;
                owl:someValuesFrom gspr:Ductile_Flow ;
              ]
            ) ;
        ] ;
    ] ;
.
gsfa:Extraction_Fault
  rdf:type owl:Class ;
  rdfs:comment "A fault whose two sides have approached each other substantially in the direction perpendicular to the fault."@en ;
  dct:source  "Froitzheim, N., Pleuger, J. & Nagel, T.J., 2006. Extraction faults. Journal of Structural Geology v28, pp. 1388-1395."@en ;
  rdfs:label "extraction fault"@en ;
  rdfs:subClassOf gsfa:Fault ;
.
gsfa:Fault
  rdf:type owl:Class ;
  rdfs:comment "A discrete surface, or zone of discrete surfaces, with some thickness, separating two rock masses across which one mass has slid past the other and characterized by brittle deformation."@en ;
  dct:source  "this vocabulary"@en ;
  rdfs:label "Fault"@en ;
  rdfs:subClassOf gsos:Fracture ;
  rdfs:subClassOf [
      rdf:type owl:Restriction ;
      owl:onProperty gsoc:hasQuality ;
      owl:someValuesFrom gsoq:Displacement ;
    ] ;
.
gsfa:Fault_Movement_Magnitude
  rdf:type owl:Class ;
  rdfs:comment "magnitude of slip or separation"@en ;
  rdfs:label "Displacement magnitude"@en ;
  rdfs:subClassOf gsoc:Physical_Quality ;
  rdfs:subClassOf [
      rdf:type owl:Restriction ;
      owl:allValuesFrom gsoq:Displacement  ;
      owl:onProperty gsoc:isQualityOf ;
    ] ;
.
gsfa:Fault_Movement_Sense
  rdf:type owl:Class ;
  rdfs:comment "Quality that specifies the relative sense of displacement (right, left, up, down) between rocks on opposites of a fault."@en ;
  rdfs:label "Fault movement sense "@en ;
  rdfs:subClassOf gsoc:Physical_Quality ;
  rdfs:subClassOf [
      rdf:type owl:Restriction ;
      owl:allValuesFrom gsoq:Displacement  ;
      owl:onProperty gsoc:isQualityOf ;
    ] ;
.
gsfa:Fault_Movement_Vector
  rdf:type owl:Class ;
  rdfs:comment "Slip vector linking piercing point on opposite sides of fault, or separation vector linking offset surface along fault trace."@en ;
  rdfs:label "Movement Vector"@en ;
  rdfs:subClassOf gsoc:Physical_Quality ;
  rdfs:subClassOf [
      rdf:type owl:Restriction ;
      owl:allValuesFrom gsoq:Displacement  ;
      owl:onProperty gsoc:isQualityOf ;
    ] ;
  rdfs:subClassOf [
      rdf:type owl:Restriction ;
      owl:onProperty gsoc:hasQuality ;
      owl:someValuesFrom gsgq:Azimuth ;
    ] ;
  rdfs:subClassOf [
      rdf:type owl:Restriction ;
      owl:onProperty gsoc:hasQuality ;
      owl:someValuesFrom gsgq:Plunge ;
    ] ;
.
gsfa:Fault_Separation
  rdf:type owl:Class ;
  rdfs:comment "a vector (magnitude and orientation) specifying the distance between the intersection of a surface on opposite sides of a displacment surface. In 3-D is the projection of a vector normal to the displaced surface into the displacment surface, but might also be specified as offset of the intersection of displacement surface and marker surface in some other profile view (e.g. horizontal/map view, or a cross section)"@en ;
  rdfs:label "Separation"@en ;
  rdfs:subClassOf gsoc:Physical_Quality ;
  rdfs:subClassOf [
      rdf:type owl:Restriction ;
      owl:allValuesFrom gsoq:Displacement  ;
      owl:onProperty gsoc:isQualityOf ;
    ] ;
.
gsfa:Fault_Slip
  rdf:type owl:Class ;
  rdfs:comment "a vector (magnitude and orientation) that links a peircing point on opposite sides of a displacement surface."@en ;
  rdfs:label "Slip"@en ;
  rdfs:subClassOf gsoc:Physical_Quality ;
  rdfs:subClassOf [
      rdf:type owl:Restriction ;
      owl:allValuesFrom gsoq:Displacement  ;
      owl:onProperty gsoc:isQualityOf ;
    ] ;
.
gsfa:Fault_Zone
  rdf:type owl:Class ;
  rdfs:comment "A material spatial feature that contains one or more fault surfaces as well as deformed rocks related to the faults located between and adjacent to the fault traces"@en ;
  rdfs:label "Fault Zone "@en ;
  rdfs:subClassOf gsoc:Material_Feature ;
  rdfs:subClassOf [
      rdf:type owl:Restriction ;
      owl:onProperty gsoc:contains ;
      owl:someValuesFrom gsfa:Fault ;
    ] ;
  rdfs:subClassOf [
      rdf:type owl:Restriction ;
      owl:onProperty gsoc:hasEssentialPart ;
      owl:someValuesFrom [
          rdf:type owl:Class ;
          owl:intersectionOf (
              gsog:Rock_Body
              [
                rdf:type owl:Restriction ;
                owl:onProperty gsoc:isOutputOf ;
                owl:someValuesFrom gsog:Deformation ;
              ]
            ) ;
        ] ;
    ] ;
  rdfs:subClassOf [
      rdf:type owl:Restriction ;
      owl:onProperty gsoc:hasQuality ;
      owl:someValuesFrom gsoq:Thickness ;
    ] ;
  rdfs:subClassOf [
      rdf:type owl:Restriction ;
      owl:onProperty gsoc:hostedBy ;
      owl:someValuesFrom gsfa:Fault ;
    ] ;
.
gsfa:Generic_Decollement_Fault
  rdf:type owl:Class ;
  rdfs:comment "A large-displacement (kilometers or tens of kilometers) shallowly dipping to subhorizontal fault or shear zone."@en ;
  dct:source  "Neuendorf et al. 2005"@en ;
  rdfs:label "decollement"@fr ;
  rdfs:label "generic decollement"@en ;
  rdfs:subClassOf gsfa:Low_Angle_Fault ;
.
gsfa:High_Angle_Fault
  rdf:type owl:Class ;
  rdfs:comment "Fault that dips at least 45 degrees over more than half of its recognized extent, for which slip or separation is not explicitly specified."@en ;
  dct:source  "CGI faulttype SKOS vocabulary 2016-10-19"@en ;
  rdfs:label "high angle fault"@en ;
  rdfs:subClassOf gsfa:Fault ;
.
gsfa:High_Angle_Normal_Fault
  rdf:type owl:Class ;
  rdfs:comment "Fault that dips at least 45 degrees over more than half of the recognized extent of the fault with the hanging wall displaced from a structurally higher position relative to footwall rocks."@en ;
  dct:source  "CGI faulttype SKOS vocabulary 2016-10-19"@en ;
  rdfs:label "high angle normal fault"@en ;
  rdfs:subClassOf gsfa:High_Angle_Fault ;
  rdfs:subClassOf gsfa:Normal_Fault ;
.
gsfa:High_Angle_Reverse_Fault
  rdf:type owl:Class ;
  rdfs:comment "Reverse fault that dips at least 45 degrees over more than half of its recognized extent, for which slip or separation is not explicitly specified."@en ;
  dct:source  "CGI faulttype SKOS vocabulary 2016-10-19"@en ;
  rdfs:label "high angle reverse"@en ;
  rdfs:subClassOf gsfa:High_Angle_Fault ;
  rdfs:subClassOf gsfa:Reverse_Fault ;
.
gsfa:Horizontal_Fault
  rdf:type owl:Class ;
  rdfs:comment "Fault that dips less than 10 degrees over more than half the recognized extent of the fault."@en ;
  dct:source  "GGIC vocabularies working group (Australia)"@en ;
  rdfs:label "horizontal fault"@en ;
  rdfs:subClassOf gsfa:Low_Angle_Fault ;
.
gsfa:Left_Normal_Fault
  rdf:type owl:Class ;
  rdfs:comment "High angle fault with slip vector that has ratio of strike-parallel to dip-parallel displacement between 10 to 1 and 1 to 10 at at least one location along the mapped trace, with left-lateral strike-parallel component and normal dip-parallel component over at least half the mapped trace of the fault."@en ;
  dct:source  "CGI faulttype SKOS vocabulary 2016-10-19"@en ;
  rdfs:label "left normal fault"@en ;
  rdfs:subClassOf gsfa:Oblique_Slip_Fault ;
.
gsfa:Left_Reverse_Fault
  rdf:type owl:Class ;
  rdfs:comment "High angle fault with slip vector that has ratio of strike-parallel to dip-parallel displacement between 10 to 1 and 1 to 10 at at least one location along the mapped trace, with left-lateral strike-parallel component and reverse dip-parallel component over at least half the mapped trace of the fault."@en ;
  dct:source  "CGI faulttype SKOS vocabulary 2016-10-19"@en ;
  rdfs:label "left reverse fault"@en ;
  rdfs:subClassOf gsfa:Oblique_Slip_Fault ;
.
gsfa:Low_Angle_Fault
  rdf:type owl:Class ;
  rdfs:comment "Fault that dips less than 45 degrees over more than half of the recognized extent of the fault."@en ;
  dct:source  "CGI faulttype SKOS vocabulary 2016-10-19"@en ;
  rdfs:label "low angle fault"@en ;
  rdfs:subClassOf gsfa:Fault ;
.
gsfa:Low_Angle_Normal_Fault
  rdf:type owl:Class ;
  rdfs:comment "Fault that dips less than 45 degrees over more than half of the recognized extent of the fault with the hanging wall displaced from a structurally higher position relative to footwall rocks."@en ;
  dct:source  "CGI faulttype SKOS vocabulary 2016-10-19"@en ;
  rdfs:label "low angle normal fault"@en ;
  rdfs:subClassOf gsfa:Low_Angle_Fault ;
  rdfs:subClassOf gsfa:Normal_Fault ;
.
gsfa:Mixed_Extraction_Fault
  rdf:type owl:Class ;
  rdfs:comment "An extraction fault with some displacement within the fault plane."@en ;
  dct:source  "Froitzheim, N., Pleuger, J. & Nagel, T.J., 2006. Extraction faults. Journal of Structural Geology v28, pp. 1388-1395."@en ;
  rdfs:label "mixed extraction fault"@en ;
  rdfs:subClassOf gsfa:Extraction_Fault ;
.
gsfa:Normal_Fault
  rdf:type owl:Class ;
  rdfs:comment "Fault with dip-parallel displacement component of slip vector more than 10 times the strike-parallel component of the slip vector over more than half recognized extent of the fault, and for which the fault dips consistently in the same direction, and for which the hanging wall has been displaced down relative to the footwall."@en ;
  dct:source  "CGI faulttype SKOS vocabulary 2016-10-19"@en ;
  rdfs:label "normal fault"@en ;
  rdfs:subClassOf gsfa:Fault ;
.
gsfa:Oblique_Slip
  rdf:type owl:Class ;
  rdfs:comment "The net slip of the fault lies between the strike and dip directions of the fault, the slip vector rakes between 10 and 80 degrees in the plane of the fault."@en ;
  dct:source  "GGIC vocabularies working group (Australia), SMR"@en ;
  rdfs:label "oblique slip"@en ;
  rdfs:subClassOf gsfa:Fault_Slip ;
.
gsfa:Oblique_Slip_Fault
  rdf:type owl:Class ;
  rdfs:comment "Fault with slip vector that has ratio of strike-parallel to dip-parallel displacement between 10 to 1 and 1 to 10 at at least one location along the mapped trace of the fault."@en ;
  dct:source  "CGI faulttype SKOS vocabulary 2016-10-19"@en ;
  rdfs:label "oblique slip fault"@en ;
  rdfs:subClassOf gsfa:Fault ;
.
gsfa:Pure_Extraction_Fault
  rdf:type owl:Class ;
  rdfs:comment "An extraction fault with no discernible displacement within the fault plane."@en ;
  dct:source  "Froitzheim, N., Pleuger, J. & Nagel, T.J., 2006. Extraction faults. Journal of Structural Geology v28, pp. 1388-1395."@en ;
  rdfs:label "pure extraction fault"@en ;
  rdfs:subClassOf gsfa:Extraction_Fault ;
.
gsfa:Reverse_Fault
  rdf:type owl:Class ;
  rdfs:comment "Fault with dip-parallel displacement component of slip vector more than 10 times the strike-parallel component of the slip vector at at least one location along the mapped trace of the fault, and the fault dips consistently in the same direction with the hanging wall displaced up relative to the footwall over at least half the mapped trace of the fault."@en ;
  dct:source  "CGI faulttype SKOS vocabulary 2016-10-19"@en ;
  rdfs:label "reverse fault"@en ;
  rdfs:subClassOf gsfa:Fault ;
.
gsfa:Right_Normal_Fault
  rdf:type owl:Class ;
  rdfs:comment "High angle fault with slip vector that has ratio of strike-parallel to dip-parallel displacement between 10 to 1 and 1 to 10 at at least one location along the mapped trace, with right-lateral strike-parallel component and normal dip-parallel component of slip over at least half the mapped trace of the fault"@en ;
  dct:source  "CGI faulttype SKOS vocabulary 2016-10-19"@en ;
  rdfs:label "right normal fault"@en ;
  rdfs:subClassOf gsfa:Oblique_Slip_Fault ;
.
gsfa:Right_Reverse_Fault
  rdf:type owl:Class ;
  rdfs:comment "High angle fault with slip vector that has ratio of strike-parallel to dip-parallel displacement between 10 to 1 and 1 to 10 at at least one location along the mapped trace, with a right-lateral strike-parallel component and reverse dip-parallel component of slip over at least half the mapped trace of the fault."@en ;
  dct:source  "CGI faulttype SKOS vocabulary 2016-10-19"@en ;
  rdfs:label "right reverse fault"@en ;
  rdfs:subClassOf gsfa:Oblique_Slip_Fault ;
.
gsfa:Scissor_Fault
  rdf:type owl:Class ;
  rdfs:comment "A fault on which there is increasing offset or separation along the strike from an initial point of no offset, with the opposite sense of offset in the opposite direction."@en ;
  dct:source  "Neuendorf et al 2005"@en ;
  rdfs:label "scissor fault"@en ;
  rdfs:subClassOf gsfa:Fault ;
.
gsfa:Sinistral_Strike_Slip_Fault
  rdf:type owl:Class ;
  rdfs:comment "Fault with left-lateral strike-parallel displacement component of slip vector more than 10 times the dip-parallel component of the slip vector at at least one location along the fault, and left-lateral displacement over more than half the mapped trace of the fault."@en ;
  dct:source  "CGI faulttype SKOS vocabulary 2016-10-19"@en ;
  rdfs:label "sinistral strike slip fault"@en ;
  rdfs:subClassOf gsfa:Strike_Slip_Fault ;
.
gsfa:Strike_Separation
  rdf:type owl:Class ;
  dct:source  "GGIC vocabularies working group (Australia)"@en ;
  rdfs:comment "planar features indicate some displacement parallel to the strike of the fault."@en ;
  rdfs:label "strike separation"@en ;
  rdfs:subClassOf gsfa:Fault_Separation ;
.
gsfa:Strike_Slip
  rdf:type owl:Class ;
  rdfs:comment "The net slip of the fault (slip vector) is parallel to the strike of the fault."@en ;
  dct:source  "GGIC vocabularies working group (Australia), this vocabulary"@en ;
  rdfs:label "strike slip"@en ;
  rdfs:subClassOf gsfa:Fault_Slip ;
.
gsfa:Strike_Slip_Fault
  rdf:type owl:Class ;
  rdfs:comment "Fault with strike-parallel displacement component of slip vector more than 10 times the dip-parallel component of the slip vector at at least one location along the mapped trace of the fault."@en ;
  dct:source  "CGI faulttype SKOS vocabulary 2016-10-19"@en ;
  rdfs:label "strike slip fault"@en ;
  rdfs:subClassOf gsfa:Fault ;
.
gsfa:Thrust_Decollement_Fault
  rdf:type owl:Class ;
  rdfs:comment "A regional-scale low-angle thrust fault."@en ;
  dct:source  "GeoScience Victoria and others"@en ;
  rdfs:label "thrust decollement"@en ;
  rdfs:subClassOf gsfa:Thrust_Fault ;
.
gsfa:Thrust_Fault
  rdf:type owl:Class ;
  rdfs:comment "Fault that dips less than 45 degrees over more than half of the recognized extent of the fault, with a hanging wall displaced from a structurally deeper position relative to footwall rocks."@en ;
  dct:source  "CGI faulttype SKOS vocabulary 2016-10-19"@en ;
  rdfs:label "thrust fault"@en ;
  rdfs:subClassOf gsfa:Low_Angle_Fault ;
  rdfs:subClassOf gsfa:Reverse_Fault ;
.
gsfa:Transcurrent_Fault
  rdf:type owl:Class ;
  rdfs:comment "A large scale strike-slip fault in which the fault surface is steeply inclined."@en ;
  dct:source  "GGIC vocabularies working group (Australia)"@en ;
  rdfs:label "transcurrent"@en ;
  rdfs:subClassOf gsfa:High_Angle_Fault ;
  rdfs:subClassOf gsfa:Strike_Slip_Fault ;
.
gsfa:Transform_Fault
  rdf:type owl:Class ;
  rdfs:comment "A variety of strike-slip fault along which the displacement suddenly stops or changes form, typically associated with mid-ocean ridges."@en ;
  dct:source  "GGIC vocabularies working group (Australia)"@en ;
  rdfs:label "transform"@en ;
  rdfs:subClassOf gsfa:Strike_Slip_Fault ;
.
gsfa:Wrench_Fault
  rdf:type owl:Class ;
  rdfs:comment "A strike slip fault in which the fault plane dips at least 45 degrees over more than half of the recognized extent of the fault."@en ;
  dct:source  "GGIC vocabularies working group (Australia)"@en ;
  rdfs:label "wrench fault"@en ;
  rdfs:subClassOf gsfa:High_Angle_Fault ;
  rdfs:subClassOf gsfa:Strike_Slip_Fault ;
.
gsfa:dextral
  rdf:type owl:Class ;
  rdfs:comment "In plan view, the side opposite the observer is displaced to the right."@en ;
  rdfs:comment "Right-lateral separation sense, in plan view, the side opposite the observer appears displaced to the right.,"@en ;
  dct:source  "GGIC vocabularies working group (Australia)"@en ;
  rdfs:label "dextral"@en ;
  rdfs:label "dextre"@fr ;
  rdfs:subClassOf gsfa:Fault_Movement_Sense ;
.
gsfa:extraction
  rdf:type owl:Class ;
  rdfs:comment "Displacement across a fault is substantially in the direction perpendicular to the fault. The fault-parallel displacement is effectively zero."@en ;
  dct:source  "Froitzheim, N., Pleuger, J. & Nagel, T.J., 2006. Extraction faults. Journal of Structural Geology v28, pp. 1388-1395."@en ;
  rdfs:label "extraction"@en ;
  rdfs:subClassOf gsfa:Fault_Movement_Sense ;
.
gsfa:no_movement_sense
  rdf:type owl:Class ;
  rdfs:comment "The fault-parallel displacement is effectively zero, as in an extraction fault."@en ;
  dct:source  "Froitzheim, N., Pleuger, J. & Nagel, T.J., 2006. Extraction faults. Journal of Structural Geology v28, pp. 1388-1395."@en ;
  rdfs:label "no movement sense"@en ;
  rdfs:subClassOf gsfa:Fault_Movement_Sense ;
.
gsfa:normal
  rdf:type owl:Class ;
  rdfs:comment "The hanging wall has been displaced down relative to the footwall, dip of fault usually 45-90 degrees."@en ;
  dct:source  "GGIC vocabularies working group (Australia)"@en ;
  rdfs:label "normal"@en ;
  rdfs:subClassOf gsfa:Fault_Movement_Sense ;
.
gsfa:normal_dextral
  rdf:type owl:Class ;
  rdfs:comment "The movement sense includes both normal and dextral components."@en ;
  dct:source  "GGIC vocabularies working group (Australia)"@en ;
  rdfs:label "normal dextral"@en ;
  rdfs:subClassOf gsfa:dextral ;
  rdfs:subClassOf gsfa:normal ;
.
gsfa:normal_sinistral
  rdf:type owl:Class ;
  rdfs:comment "The movement sense includes both normal and sinistral components."@en ;
  dct:source  "GGIC vocabularies working group (Australia)"@en ;
  rdfs:label "normal sinistral"@en ;
  rdfs:subClassOf gsfa:normal ;
  rdfs:subClassOf gsfa:sinistral ;
.
gsfa:ontology
  rdf:type owl:Ontology ;
  rdfs:comment "This file contains the 2016 SKOS-RDF version of the CGI Fault Type, Fault Movement Sense and Fault Movement Type vocabulary. Compilation and review in MS Excel spreadsheet, converted to MS Excel for SKOS generation using SKOS_for_GA_from_XLS_2016.03.xslt"@en ;
  rdfs:comment "This ontology includes extensions for describing faults in more detail. (ie, a summary of movement type and orientation) as defined by the IUGS Commission for Geoscience Information (CGI) Geoscience Terminology Working Group. Although the terms in this vocabulary are in common usage with definitions in standard texts or glossaries like Neuendorf et al. (2005), the definitions here attempt to establish unambiguous criteria to distinguish the categories, and are thus listed with this vocabulary as the source."@en ;
  rdfs:comment "dct:creator--  CGI Geoscience Terminology Working Group; OWL conversion by Stephen Richard for Loop3D project"@en ;
  rdfs:comment "dct:date--  2016-10-19"@en ;
  rdfs:comment "dct:modified-- 2020-01-29"@en ;
  rdfs:label "Fault"@en ;
  owl:imports gsoc:ontology ;
  owl:imports gspr:ontology ;
  owl:imports gsgq:ontology ;
  owl:imports gsog:ontology ;
  owl:imports gsoq:ontology ;
  owl:imports gsos:ontology ;
.
gsfa:reverse
  rdf:type owl:Class ;
  rdfs:comment "The hanging wall has been displaced up relative to the footwall, dip of fault usually greater than 45 degrees."@en ;
  dct:source  "GGIC vocabularies working group (Australia)"@en ;
  rdfs:label "inverse"@fr ;
  rdfs:label "reverse"@en ;
  rdfs:subClassOf gsfa:Fault_Movement_Sense ;
.
gsfa:reverse_dextral
  rdf:type owl:Class ;
  rdfs:comment "The movement sense includes both reverse and dextral components."@en ;
  dct:source  "GGIC vocabularies working group (Australia)"@en ;
  rdfs:label "reverse dextral"@en ;
  rdfs:subClassOf gsfa:dextral ;
  rdfs:subClassOf gsfa:reverse ;
.
gsfa:reverse_sinistral
  rdf:type owl:Class ;
  rdfs:comment "The movement sense includes both reverse and sinistral components."@en ;
  dct:source  "GGIC vocabularies working group (Australia)"@en ;
  rdfs:label "reverse sinistral"@en ;
  rdfs:subClassOf gsfa:reverse ;
  rdfs:subClassOf gsfa:sinistral ;
.
gsfa:scissor_movement
  rdf:type owl:Class ;
  rdfs:comment "A fault on which there is increasing offset or separation along the strike from an initial point of no offset, with reverse offset in the opposite direction."@en ;
  dct:source  "Neuendorf et al 2005"@en ;
  rdfs:label "scissor"@en ;
  rdfs:subClassOf gsfa:Fault_Movement_Sense ;
.
gsfa:sinistral
  rdf:type owl:Class ;
  rdfs:comment "In plan view the side opposite the observer is displaced to the left."@en ;
  dct:source  "GGIC vocabularies working group (Australia)"@en ;
  rdfs:label "sinistral"@en ;
  rdfs:subClassOf gsfa:Fault_Movement_Sense ;
.
